%!TEX root = ./main.tex

\section{Online \emph{non-linear} covering with experts} \label{sec:convex-proofs}

\subsection{Missing proofs from the algorithm's performance analysis}
As $w^{t}$ is the locally optimal solution of the non-linear program and ($\theta^t,\ \chi_{i},\ \nu_{i}^{t}$) is the locally optimal solution of its dual, the following Karush-Kuhn-Tucker (KKT) and complementary slackness conditions hold (Theorem 12.1 on page 321 \cite{NocedalWright:FirstOrderOptimalityConditions}).

\begin{align*}
   \biggl[ \sum_{i=1}^{n} a_{i}^{t} \biggl( \sum_{k=1}^{K}  \hat{s}_{i,k}^{t} w_{i,k}^{t} \biggr) - 1 \biggr] \theta^{t} &= 0 \qquad \forall \ t \\
   \biggl[ \sum_{k=1}^{K}  w_{i,k}^{t}  - 1 \biggr] \chi_{i} &= 0 \qquad \forall\ i, t \\
   \biggl[ \sum_{k=1}^{K}  s_{i,k}^{t} w_{i,k}^{t} \biggr] \nu_{i}^{t} &= 0 \qquad \forall\ i, t \\
%
 s_{i,k}^{t} \biggl[  \nabla_{i} f(x^{t-1}) + L\biggl( \sum_{k=1}^{K} s_{i,k}^{t} w_{i,k}^{t} + \delta_{i}^{t} - \sum_{k=1}^{K} s_{i,k}^{t-1} w_{i,k}^{t-1} - \delta_{i}^{t-1} \biggr) \biggr] \ln \left( \frac{\sum_{k=1}^{K} s_{i,k}^{t} w_{i,k}^{t} + \delta_{i}^{t}}{\sum_{k=1}^{K}  s_{i,k}^{t-1}w_{i,k}^{t-1}  + \delta_{i}^{t-1}} \right) \\
        - a_{i}^{t} \hat{s}_{i,k}^{t} \theta^{t} - \chi_{i} - s_{i,k}^{t} \nu_{i}^{t} &= 0	\qquad \forall\ i,k,t \\
    %
    \theta^{t}, \chi_{i}, \nu_{i}^{t} &\geq 0 \qquad \forall\ i, t
\end{align*}

Moreover, if $\sum_{k} w_{i,k}^{t} s_{i,k}^{t} > 0$, meaning that $\nu_{i}^{t} = 0$, then
\begin{align}	\label{eq:KKT2}
 s_{i,k}^{t} \biggl[  \nabla_{i} f(x^{t-1}) + L\biggl( \sum_{k=1}^{K} s_{i,k}^{t} w_{i,k}^{t} + \delta_{i}^{t} - \sum_{k=1}^{K} s_{i,k}^{t-1} w_{i,k}^{t-1} - \delta_{i}^{t-1} \biggr) \biggr] \ln & \left( \frac{\sum_{k=1}^{K} s_{i,k}^{t} w_{i,k}^{t} + \delta_{i}^{t}}{\sum_{k=1}^{K}  s_{i,k}^{t-1}w_{i,k}^{t-1}  + \delta_{i}^{t-1}} \right) \notag \\
        &- a_{i}^{t} \hat{s}_{i,k}^{t} \theta^{t} - \chi_{i}^{t} = 0
\end{align}


\paragraph{Dual variables and feasibility.} We set the dual variables of the reformulation of our \texttt{LIN-COMB} benchmark based on the dual variables of the non-linear program used inside the algorithm. The dual formulation is visible on \cref{fig:reformulation}. The constants $\lambda$ and $\mu$ correspond to the $(\lambda,\mu)$-local-smoothness, and $L$ to the L-gradient-Lipschitz of $f$ (see the definitions at \cref{sec:f-properties}).

\begin{align*}
    \alpha^{t} &= \frac{1}{\lambda}  \biggl( \theta^{t} + \sum_{i=1}^{n} \chi_{i} \biggr), \\
    %
    \beta_{i}^{t} &= \frac{1}{\lambda} \biggl[  \nabla_{i} f(x^{t-1}) + L\biggl( \sum_{k=1}^{K} s_{i,k}^{t} w_{i,k}^{t} + \delta_{i}^{t} - \sum_{k=1}^{K} s_{i,k}^{t-1} w_{i,k}^{t-1} - \delta_{i}^{t-1} \biggr)  \biggr] \ln \left( \frac{\sum_{k=1}^{K} s_{i,k}^{t} w_{i,k}^{t} + \delta_{i}^{t}}{\sum_{k=1}^{K}  s_{i,k}^{t-1}w_{i,k}^{t-1}  + \delta_{i}^{t-1}} \right) \\
    %
    \xi_{S}^{t} &= \frac{1}{\lambda} \sum_{i \in S} \nabla_{i} f(x^{t-1}) \ln \left( \frac{(1 + 1/K) \cdot \max_{t'} \sum_{k=1}^{K} s_{i,k}^{t'}}{\sum_{k=1}^{K}  s_{i,k}^{t-1}w_{i,k}^{t-1}  + \delta_{i}^{t-1}} \right) - \frac{\mu}{\lambda} \ln(K\rho)  f(x^{t-1})\\
    %
    \gamma^{t} &= -  \frac{1}{\lambda} \sum_{i=1}^{n} \biggl[  \nabla_{i} f(x^{t-1}) + L\biggl( \sum_{k=1}^{K} s_{i,k}^{t} w_{i,k}^{t} + \delta_{i}^{t} - \sum_{k=1}^{K} s_{i,k}^{t-1} w_{i,k}^{t-1} - \delta_{i}^{t-1} \biggr) \biggr]  \ln \left( \frac{\sum_{k=1}^{K} s_{i,k}^{t} w_{i,k}^{t} + \delta_{i}^{t}}{\sum_{k=1}^{K}  s_{i,k}^{t-1}w_{i,k}^{t-1}  + \delta_{i}^{t-1}} \right) \\
        & \quad - \frac{1}{\lambda} \sum_{i=1}^{n} \biggl[ \nabla_{i} f(x^{t}) \ln \left( \frac{(1 + 1/K) \cdot \max_{t'} \sum_{k=1}^{K} s_{i,k}^{t'}}{\sum_{k=1}^{K}  s_{i,k}^{t}w_{i,k}^{t}  + \delta_{i}^{t}} \right) -  \nabla_{i} f(x^{t-1}) \ln \left( \frac{(1 + 1/K) \cdot \max_{t'} \sum_{k=1}^{K} s_{i,k}^{t'}}{\sum_{k=1}^{K}  s_{i,k}^{t-1}w_{i,k}^{t-1}  + \delta_{i}^{t-1}} \right) \biggr] \\
    & \quad + \frac{\mu}{\lambda} \ln(K\rho) f(x^{t}) - \frac{\mu}{\lambda} \ln(K\rho) f(x^{t-1})
\end{align*}
%
Recall that $\rho = \max_{i, t',t''} \left\{\frac{\sum_{k=1}^{K} s_{i,k}^{t'}}{\sum_{k=1}^{K} s_{i,k}^{t''}} : \sum_{k=1}^{K} s_{i,k}^{t''} > 0 \right\}$.

\begin{lemma} \label{lem:convex-covering-feasibility}
The original covering problem's $x_{i}^{t}$ solution set by the algorithm and the dual variables $(\alpha^{t}, \beta_{i}^{t}, \xi_S^t, \gamma^t)$ of the reformulated \texttt{LIN-COMB} benchmark are feasible up to a factor of $\ln (K\rho)$.
\end{lemma}
%
\begin{proof}
We first prove that the $x_{i}^{t}$ variables satisfy the covering constraints by induction. At time~0, no constraint has been released yet, and every variable is set to 0. This all-zero solution is feasible. Let us assume that the algorithm provides feasible solutions up to time $t-1$. At time~$t$, the algorithm maintains the inequality $x_{i}^{t} \geq x_{i}^{t-1}$, so all constraints $t'$ where $t' < t$ are satisfied. Besides, $x_{i}^{t}$ is always at least
$\sum_{k} w_{i,k}^{t} s_{i,k}^{t}$, which is larger than $\sum_{k} w_{i,k}^{t} \hat{s}_{i,k}^{t}$ since $s_{i,k}^{t} \geq \hat{s}_{i,k}^{t}$
for all $i,k$ due to the preprocessing step. Hence, constraint $t$ is also satisfied, formally,
$$
\sum_{i=1}^{n} a_{i}^{t} x_{i}^{t}  \geq \sum_{i=1}^{n} a_{i}^{t} \biggl( \sum_{k=1}^{K} \hat{s}_{i,k}^{t} w_{i,k}^{t} \biggr) \geq 1.
$$

In the remaining part of the proof, we show the feasibility of the dual solution. The dual constraints are visible on \cref{fig:reformulation}.
The first constraint follows from the KKT conditions and from the fact that $\sum_{i} a_i^{t} \hat{s}_{i,k}^{t} = 1$.
The second constraint is satisfied up to a factor of $\ln (K\rho)$ because
%
\begin{align*}
\xi_{S}^{t} &= \frac{1}{\lambda} \sum_{i \in S} \nabla_{i} f(x^{t-1}) \ln \left( \frac{(1 + 1/K) \cdot \max_{t'} \sum_{k=1}^{K} s_{i,k}^{t'}}{\sum_{k=1}^{K}  s_{i,k}^{t-1}w_{i,k}^{t-1}  + \delta_{i}^{t-1}} \right) - \frac{\mu}{\lambda} \ln(K\rho) f(x^{t-1})  \\
&\leq \frac{1}{\lambda} \sum_{i \in S} \nabla_{i} f(x^{t-1}) \ln(K\rho)  - \frac{\mu}{\lambda} \ln(K\rho) f(x^{t-1})
\leq  \ln(K\rho) c_S
\end{align*}
%
where the last inequality holds due to the $(\lambda,\mu)$-local-smoothness. Important: after down-scaling the variables by a factor of $\ln (K\rho)$, the second dual constraint holds.

The last constraint is satisfied due to the definition of the dual variables. We need
\begin{align*}
  \sum_{i \in S}\beta_{i}^{t} + \gamma^{t} - \xi_{S}^{t} + \xi_{S}^{t+1}  &\leq 0\\
  \sum_{i \in S}\beta_{i}^{t} - \xi_{S}^{t} + \xi_{S}^{t+1}  &\leq -\gamma^{t}
\end{align*}
%
to hold. We can rewrite $\gamma^{t}$ as follows:
\begin{align*}
    \gamma^{t} &= -  \frac{1}{\lambda} \sum_{i=1}^{n} \biggl[ L\biggl( \sum_{k=1}^{K} s_{i,k}^{t} w_{i,k}^{t} + \delta_{i}^{t} - \sum_{k=1}^{K} s_{i,k}^{t-1} w_{i,k}^{t-1} - \delta_{i}^{t-1} \biggr) \biggr]  \ln \left( \frac{\sum_{k=1}^{K} s_{i,k}^{t} w_{i,k}^{t} + \delta_{i}^{t}}{\sum_{k=1}^{K}  s_{ik}^{t-1}w_{i,k}^{t-1}  + \delta_{i}^{t-1}} \right) \\
    	& \quad - \frac{1}{\lambda} \sum_{i=1}^{n} \biggl[ \nabla_{i} f(x^{t}) - \nabla_{i} f(x^{t-1}) \biggr] \ln \left( \frac{(1 + 1/K) \cdot \max_{t'} \sum_{k=1}^{K} s_{i,k}^{t'}}{\sum_{k=1}^{K}  s_{ik}^{t}w_{i,k}^{t}  + \delta_{i}^{t}} \right)  \\
	& \quad + \frac{\mu}{\lambda} \ln(K\rho) f(x^{t}) - \frac{\mu}{\lambda} \ln(K\rho) f(x^{t-1})
\end{align*}
%
Now let us fix an arbitrary set $S$. Then, following the simplified form of $\gamma^t$, we have
\begin{align*}
    -\gamma^{t} &\geq     \frac{1}{\lambda} \sum_{i \in S} \biggl[ L\biggl( \sum_{k=1}^{K} s_{i,k}^{t} w_{i,k}^{t} + \delta_{i}^{t} - \sum_{k=1}^{K} s_{i,k}^{t-1} w_{i,k}^{t-1} - \delta_{i}^{t-1} \biggr) \biggr]  \ln \left( \frac{\sum_{k=1}^{K} s_{i,k}^{t} w_{i,k}^{t} + \delta_{i}^{t}}{\sum_{k=1}^{K}  s_{ik}^{t-1}w_{i,k}^{t-1}  + \delta_{i}^{t-1}} \right) \\
            & \quad + \frac{1}{\lambda} \sum_{i \in S} \biggl[ \nabla_{i} f(x^{t}) - \nabla_{i} f(x^{t-1}) \biggr] \ln \left( \frac{(1 + 1/K) \cdot \max_{t'} \sum_{k=1}^{K} s_{i,k}^{t'}}{\sum_{k=1}^{K}  s_{ik}^{t}w_{i,k}^{t}  + \delta_{i}^{t}} \right)  \\
        & \quad - \frac{\mu}{\lambda} \ln(K\rho) f(x^{t}) + \frac{\mu}{\lambda} \ln(K\rho) f(x^{t-1})
\end{align*}
%
since the terms in the first two lines are positive and we restrict the sum to a subset. In particilar, $\nabla_{i} f(x^{t}) \geq \nabla_{i} f(x^{t-1})$ by assumption of function $f$, and either $\sum_{k=1}^{K} s_{i,k}^{t} w_{i,k}^{t} + \delta_{i}^{t} \geq \sum_{k=1}^{K} s_{i,k}^{t} w_{i,k}^{t-1} + \delta_{i}^{t-1}$ and the logarithm term is non-negative, or $\sum_{k=1}^{K} s_{i,k}^{t} w_{i,k}^{t} + \delta_{i}^{t} < \sum_{k=1}^{K} s_{i,k}^{t} w_{i,k}^{t-1} + \delta_{i}^{t-1}$ and the logarithm term is also negative, making their product non-negative.
%
We have to show that the following is true to satisfy the third constraint:
\begin{align*}
    \sum_{i \in S} & \beta_{i}^{t} - \xi_{S}^{t} + \xi_{S}^{t+1} \\
    %
    & = \sum_{i \in S} \frac{1}{\lambda} \biggl[  \nabla_{i} f(x^{t-1}) + L\biggl( \sum_{k=1}^{K} s_{i,k}^{t} w_{i,k}^{t} + \delta_{i}^{t} - \sum_{k=1}^{K} s_{i,k}^{t-1} w_{i,k}^{t-1} - \delta_{i}^{t-1} \biggr) \biggr] \ln \left( \frac{\sum_{k=1}^{K} s_{i,k}^{t} w_{i,k}^{t} + \delta_{i}^{t}}{\sum_{k=1}^{K}  s_{i,k}^{t-1}w_{i,k}^{t-1}  + \delta_{i}^{t-1}} \right) \\
        & \quad - \frac{1}{\lambda} \sum_{i \in S} \nabla_{i} f(x^{t-1}) \ln \left( \frac{(1 + 1/K) \cdot \max_{t'} \sum_{k=1}^{K} s_{i,k}^{t'}}{\sum_{k=1}^{K}  s_{i,k}^{t-1}w_{i,k}^{t-1}  + \delta_{i}^{t-1}} \right) + \frac{\mu}{\lambda} \ln(K\rho)  f(x^{t-1}) \\
        & \quad + \frac{1}{\lambda} \sum_{i \in S} \nabla_{i} f(x^{t}) \ln \left( \frac{(1 + 1/K) \cdot \max_{t'} \sum_{k=1}^{K} s_{i,k}^{t'}}{\sum_{k=1}^{K}  s_{i,k}^{t}w_{i,k}^{t}  + \delta_{i}^{t}} \right) - \frac{\mu}{\lambda} \ln(K\rho)  f(x^{t}) \\
       %
    & =     \frac{1}{\lambda} \sum_{i \in S} \biggl[ L\biggl( \sum_{k=1}^{K} s_{i,k}^{t} w_{i,k}^{t} + \delta_{i}^{t} - \sum_{k=1}^{K} s_{i,k}^{t-1} w_{i,k}^{t-1} - \delta_{i}^{t-1} \biggr) \biggr]  \ln \left( \frac{\sum_{k=1}^{K} s_{i,k}^{t} w_{i,k}^{t} + \delta_{i}^{t}}{\sum_{k=1}^{K}  s_{ik}^{t-1}w_{i,k}^{t-1}  + \delta_{i}^{t-1}} \right) \\
            & \quad + \frac{1}{\lambda} \sum_{i \in S} \biggl[ \nabla_{i} f(x^{t}) - \nabla_{i} f(x^{t-1}) \biggr] \ln \left( \frac{(1 + 1/K) \cdot \max_{t'} \sum_{k=1}^{K} s_{i,k}^{t'}}{\sum_{k=1}^{K}  s_{ik}^{t}w_{i,k}^{t}  + \delta_{i}^{t}} \right)  \\
            & \quad - \frac{\mu}{\lambda} \ln(K\rho) f(x^{t}) + \frac{\mu}{\lambda} \ln(K\rho) f(x^{t-1}) \\
    & \leq - \gamma^t
\end{align*}
where the second equality holds due to $\log(a/b) - \log(a/c) = \log(c/b)$.

It remains to show that $\alpha^t$ and $\beta_i^t$ are positive. Due to the KKT conditions both variables are always positive, so the lemma holds.
\end{proof}

\begin{theorem} \label{convex-covering-theorem}
Algorithm 2 is $O(\ln(K \rho)) \frac{\lambda}{1 - \mu \ln (K\rho)}$-competitive with the \texttt{LIN-COMB} benchmark.
\end{theorem}
%
\begin{proof} \cref{lem:convex-covering-feasibility} proved that our algorithm creates feasible solutions for the original covering problem and for the dual problem of the reformulated \texttt{LIN-COMB} benchmark. We show that the algorithm's solution increases the primal objective value of the original covering problem by at most $O(\ln(K \rho))$ times the value of the dual solution, which serves as the lower bound on the \texttt{LIN-COMB} benchmark - the best linear combination of the experts' solutions.

\begin{align}
&f(x^{t}) - f(x^{t-1}) \leq \nabla f(x^{t-1}) (x^{t} - x^{t-1}) + \frac{2L}{2} \|x^{t} - x^{t-1} \|^{2} \\
%
&\leq \sum_{i: x_{i}^{t} > x_{i}^{t-1}} \bigl[ \nabla_{i} f(x^{t-1}) + L(x_{i}^{t} - x_{i}^{t-1}) \bigr] (x_{i}^{t} - x_{i}^{t-1}) &&  \notag \\
%
&\leq \sum_{i: x_{i}^{t} > x_{i}^{t-1}} \bigl[ \nabla_{i} f(x^{t-1}) + L(x_{i}^{t} - x_{i}^{t-1}) \bigr](x_{i}^{t} + \delta_{i}^{t}) \ln \left(\frac{x_{i}^{t} + \delta_{i}^{t}}{x_{i}^{t-1} + \delta_{i}^{t}} \right) \\
%
&\leq \sum_{i: x_{i}^{t} > x_{i}^{t-1}} \bigl[ \nabla_{i} f(x^{t-1}) + L(x_{i}^{t} - x_{i}^{t-1}) \bigr] (x_{i}^{t} + \delta_{i}^{t}) \ln \left(\frac{x_{i}^{t} + \delta_{i}^{t}}{x_{i}^{t-1} + \delta_{i}^{t-1}} \right) \\
%
&= \sum_{i: x_{i}^{t} > x_{i}^{t-1}} \bigl[ \nabla_{i} f(x^{t-1}) + L(x_{i}^{t} - x_{i}^{t-1}) \bigr] \left[ \left(\sum_{k=1}^{K}  s_{i,k}^{t} w_{i,k}^{t} + \frac{1}{K} \sum_{k=1}^{K} s_{i,k}^{t} \right)
            \ln \left(\frac{ \sum_{k=1}^{K}  s_{i,k}^{t} w_{i,k}^{t} + \delta_{i}^{t}}{x_{i}^{t-1} + \delta_{i}^{t-1}}  \right) \right]\\
%
&\leq \sum_{i: x_{i}^{t} > x_{i}^{t-1}} \bigl[ \nabla_{i} f(x^{t-1}) + L(x_{i}^{t} - x_{i}^{t-1}) \bigr] \left[ \left(\sum_{k=1}^{K}  s_{i,k}^{t} w_{i,k}^{t} + \frac{1}{K} \sum_{k=1}^{K} s_{i,k}^{t} \right)
            \ln \left(\frac{ \sum_{k=1}^{K}  s_{i,k}^{t} w_{i,k}^{t} + \delta_{i}^{t}}{\sum_{k=1}^{K}  s_{i,k}^{t-1} w_{i,k}^{t-1} + \delta_{i}^{t-1}}  \right) \right]\\
%
&= \sum_{i: x_{i}^{t} > x_{i}^{t-1}} \sum_{k=1}^{K} (w_{i,k}^{t} + 1/K) s_{i,k}^{t} \bigl[ \nabla_{i} f(x^{t-1}) + L(x_{i}^{t} - x_{i}^{t-1}) \bigr]
            \ln \left(\frac{ \sum_{k=1}^{K} s_{i,k}^{t} w_{i,k}^{t}  + \delta_{i}^{t}}{\sum_{k=1}^{K}  s_{i,k}^{t-1} w_{i,k}^{t-1}  + \delta_{i}^{t-1}}  \right) \notag \\
%
&\leq \sum_{i: x_{i}^{t} > x_{i}^{t-1}} \sum_{k=1}^{K} (w_{i,k}^{t} + 1/K) s_{i,k}^{t} \biggl[ \nabla_{i} f(x^{t-1}) + L\biggl( \sum_{k=1}^{K} s_{i,k}^{t} w_{i,k}^{t} + \delta_{i}^{t} - \sum_{k=1}^{K} s_{i,k}^{t-1} w_{i,k}^{t-1} - \delta_{i}^{t-1} \biggr) \biggr] \cdot \notag \\
    &\hspace{5cm} \ln \left(\frac{ \sum_{k=1}^{K} s_{i,k}^{t} w_{i,k}^{t}  + \delta_{i}^{t}}{\sum_{k=1}^{K}  s_{i,k}^{t-1} w_{i,k}^{t-1}  + \delta_{i}^{t-1}}  \right) \\
%
&=  \sum_{i: x_{i}^{t} > x_{i}^{t-1}} \sum_{k=1}^{K} (w_{i,k}^{t} + 1/K) \biggl( a_{i}^{t} \hat{s}_{i,k}^{t} \theta^{t} + \chi_{i}^{t} \biggr)  \\
%
&\leq \sum_{i=1}^{n} \sum_{k=1}^{K} (w_{i,k}^{t} + 1/K) \biggl( a_{i}^{t} \hat{s}_{i,k}^{t} \theta^{t} + \chi_{i}^{t} \biggr) \notag \\
%
&= \sum_{i=1}^{n} a_{i}^{t} \biggl(\sum_{k=1}^{K} w_{i,k}^{t} \hat{s}_{i,k}^{t} \biggr) \theta^t + \sum_{i=1}^{n} \biggl( \sum_{k=1}^{K} w_{i,k}^{t} \biggr) \chi_{i}^{t}
+ \frac{1}{K}  \sum_{k=1}^{K} \biggl( \sum_{i=1}^{n} a_{i}^{t}  \hat{s}_{i,k}^{t}  \biggr) \theta^t + \frac{1}{K} \sum_{k=1}^{K} \sum_{i=1}^{n} \chi_{i}^{t} 		\notag \\
%
&= 2 \theta^{t} + 2\sum_{i=1}^{n} \chi_{i}^{t} \\
%
&= 2\lambda \cdot \alpha^{t}	\notag
\end{align}
%
The above corresponding transformations hold since:
\begin{compactenum}[(1)]
    \setcounter{enumi}{8}
    \item holds as $f$ is $2L$-smooth;
    \item follows from the inequality $a - b \leq a \ln(a/b)$ for all $0 < b \leq a$;
    \item holds since $\delta_{i}^{t} \geq \delta_{i}^{t-1}$ (because $s_{i,k}^{t} \geq s_{i,k}^{t-1}$ for all $i,k,t$);
    \item is valid because $x_{i}^{t} > x_{i}^{t-1}$, so $x_{i}^{t} = \sum_{k=1}^{K}  s_{i,k}^{t} w_{i,k}^{t}$;
    \item is by the design of the algorithm: $x_{i}^{t-1} \geq \sum_{k=1}^{K}  s_{i,k}^{t-1} w_{i,k}^{t-1}$;
    %\setcounter{enumi}{5}
    \item since again, $x_{i}^{t} > x_{i}^{t-1} \geq 0$, we have $x_{i}^{t} = \sum_{k=1}^{K}  s_{i,k}^{t} w_{i,k}^{t}$ and
    	it always holds that $x_{i}^{t-1} \geq \sum_{k=1}^{K}  s_{i,k}^{t-1} w_{i,k}^{t-1}$;
    \item since given that $x_{i}^{t} > x_{i}^{t-1} \geq 0$ (so $\sum_{k=1}^{K}  s_{i,k}^{t} w_{i,k}^{t} = x_{i}^{t} > 0$), the KKT condition (\ref{eq:KKT2}) applies;
    \item is true due to the complementary slackness conditions
        and that $\sum_{i=1}^{n} a_{i}^{t}  \hat{s}_{i,k}^{t} = 1$.
\end{compactenum}


\noindent The objective of the dual includes $\sum_{t = 1}^{T} \gamma^{t}$ as well, so it remains to bound this sum. Recall the simplified version of $\gamma^t$:
\begin{align*}
    \gamma^{t} &= -  \frac{1}{\lambda} \sum_{i=1}^{n} \biggl[  L\biggl( \sum_{k=1}^{K} s_{i,k}^{t} w_{i,k}^{t} + \delta_{i}^{t} - \sum_{k=1}^{K} s_{i,k}^{t-1} w_{i,k}^{t-1} - \delta_{i}^{t-1} \biggr) \biggr]  \ln \left( \frac{\sum_{k=1}^{K} s_{i,k}^{t} w_{i,k}^{t} + \delta_{i}^{t}}{\sum_{k=1}^{K}  s_{ik}^{t-1}w_{i,k}^{t-1}  + \delta_{i}^{t-1}} \right) \\
    	& \quad - \frac{1}{\lambda} \sum_{i=1}^{n} \biggl[ \nabla_{i} f(x^{t}) - \nabla_{i} f(x^{t-1}) \biggr] \ln \left( \frac{(1 + 1/K) \cdot \max_{t'} \sum_{k=1}^{K} s_{i,k}^{t'}}{\sum_{k=1}^{K}  s_{ik}^{t}w_{i,k}^{t}  + \delta_{i}^{t}} \right)  \\
	& \quad + \frac{\mu}{\lambda} \ln(K\rho) f(x^{t}) - \frac{\mu}{\lambda} \ln(K\rho) f(x^{t-1})
\end{align*}
%
Since $f$ is $2L$-smooth with respect to the $\ell_{2}$-norm, we can observe that
\begin{align*}
\sum_{i=1}^{n} (\nabla_{i} f(x^{t}) -  \nabla_{i} f(x^{t-1}) \ln \left( \frac{(1 + 1/K) \cdot \max_{t'} \sum_{k=1}^{K} s_{i,k}^{t'}}{\sum_{k=1}^{K}  s_{i,k}^{t}w_{i,k}^{t}  + \delta_{i}^{t}} \right)
\leq \ln(K\rho) 2L\sqrt{n} \sum_{i=1}^{n} (x_{i}^{t} - x_{i}^{t-1})
\end{align*}
%
and after bounding the following term
%
\begin{align*}
2\biggl( \sum_{k=1}^{K} s_{i,k}^{t} w_{i,k}^{t}  - x_{i}^{t-1} \biggr) \ln \left( \frac{\sum_{k=1}^{K} s_{i,k}^{t} w_{i,k}^{t} + \delta_{i}^{t}}{\sum_{k=1}^{K}  s_{i,k}^{t-1}w_{i,k}^{t-1}  + \delta_{i}^{t-1}} \right)
\leq \ln(K\rho) (x_{i}^{t} - x_{i}^{t-1})
\end{align*}
%
we get that
\begin{align*}
\sum_{t=1}^{T} \gamma^{t} &\geq - \frac{\mu \ln (K\rho)}{\lambda} f(x^{T}) - \ln(K\rho) \frac{4L}{\lambda} \sqrt{n} \sum_{t=1}^{T} \sum_{i=1}^{n} (x_{i}^{t} - x_{i}^{t-1}) \\
&\geq - \frac{\mu \ln (K\rho)}{\lambda} f(x^{T}) - \ln(K\rho) \frac{4L}{\lambda} \sqrt{n} \sum_{i=1}^{n} x_{i}^{T}.
\end{align*}
Considering both parts of the proof so far, we bound the dual objective as follows:
\begin{align*}
\sum_{t=1}^{T} (\alpha^{t} + \gamma^{t}) \geq \frac{1/2-\mu\ln (K\rho)}{\lambda} f(x^{T}) - \ln(K\rho) \frac{4L}{\lambda} \sqrt{n} \sum_{i=1}^{n} x_{i}^{T}
\end{align*}
In $0-1$ optimization, $x_{i}^{T} \leq 1$.
Hence, the theorem follows.
\end{proof}
